<?xml version='1.0' encoding='UTF-8'?>

<!--copied by libby - same at 2001-06-27

Michael Arick

2001-06-18

This RDF Schema represents a hybrid of two RDF schema written by Michael Arick
and Libby Miller.  These schema are intended to implement calendar/scheduling
data (see iCalendar, calsh working group, IETF).

-->
<!--ENTITY iCalendar 
'http://ilrt.org/discovery/2001/06/schemas/ical-full/hybrid.rdf#' -->
<!--ENTITY xx 'http://www.w3.org/2001/XMLSchema#'-->

<!DOCTYPE rdf:RDF [
 	 <!ENTITY rdf 'http://www.w3.org/1999/02/22-rdf-syntax-ns#'>
	 <!ENTITY iCalendar ''>
 	 <!ENTITY rdfs 'http://www.w3.org/2000/01/rdf-schema#'>
         <!ENTITY xmlsdt 'http://www.w3.org/2001/XMLSchema#'>
         <!ENTITY dc 'http://purl.org/dc/elements/1.1/'>
         <!ENTITY foaf 'http://xmlns.com/foaf/0.1/'> 
 ]>


<rdf:RDF xmlns:rdf="&rdf;"
 	 xmlns:iCalendar=""
	 xmlns:rdfs="&rdfs;"
         xmlns:dc="&dc;"

>

<rdf:Description rdf:about="" 
      dc:creator="Michael Arick"
      dc:contributor="Libby Miller" 
      dc:title="Hybrid iCal-like RDF Schema"
      dc:description="This RDF Schema represents a hybrid of two RDF schema 
written by Michael Arick and Libby Miller.  These schema are intended to implement
calendar/scheduling data (see iCalendar, calsh working group, IETF)."
      dc:date="2001-06-17"/>


<!--Simple Data Types-->
<!-- The rdf:about="&iCalendar;.." was replaced by rdf:ID=".." -->

<rdfs:Class rdf:ID="BINARY"
 rdfs:label="binary"
 rdfs:comment="Used to identify properties that contain a character encoding of inline binary data.">
 <rdfs:subClassOf rdf:resource="&xmlsdt;base64binary"/>
</rdfs:Class>

<rdfs:Class rdf:ID="BOOLEAN"
 rdfs:label="boolean"
 rdfs:comment="A boolean data type. The iCalendar rfc 2445 defines it as a literal, either TRUE or FALSE (case insensitive) ">
 <rdfs:subClassOf rdf:resource="&xmlsdt;boolean" />
</rdfs:Class>


<rdfs:Class
 rdf:ID="CAL-ADDRESS"
 rdfs:label="Calendar user address"
 rdfs:comment="Used to identify properties that contain a calendar user
address. When used to address an Internet email transport address for a
calendar user, the value must be a MAILTO uri" >

<!-- this should distinguish between a user and their address. It is used in
RFC 2445 as a person or resource identifier. -->

<rdfs:subClassOf rdf:resource="&xmlsdt;anyURL" />
</rdfs:Class>

<!-- TimeEntry is a superclass of DATE and DATE-TIME since many properties
take either.-->

<rdfs:Class 
 rdf:ID="TimeEntry"
 rdfs:label="TimeEntry"
 rdfs:comment="Date or Date-Time"/>

<rdfs:Class
 rdf:ID="DATE"
 rdfs:label="Date"
 rdfs:comment=" A value type which is used to identify values that specify a
 calendar date.">

<!-- year (4 digits) month (2 digits) date (2 digits) 
Is there a Daml/xsd date datatype? 
The XML Schema datatypes includes this kind of date.
-->
<rdfs:subClassOf rdf:resource="&xmlsdt;date" />
<rdfs:subClassOf rdf:resource="#TimeEntry"/>
<rdfs:subClassOf rdf:resource="#TriggerEntry"/>
</rdfs:Class>

<!-- The class TriggerEntry has not been defined before. For this, it is
typically defined -->
<rdfs:Class rdf:ID="TriggerEntry"
 rdfs:label="TriggerEntry"/>

<rdfs:Class
rdf:ID="DATE-TIME"
 rdfs:label="Date-time"
 rdfs:comment=" A value type which is used to identify values that specify a
precise calendar date and time of day. ">

<!-- I am unsure if this should be a property or a class; B-L regards it as
a class. RFC 2445 has a specific syntax for writing it down though. The
SKICal RDF notes and the RSS events have a string as a date. Note really
feasible with timezones, etc though. Suggest we go with rdf:value, like the
DC model in RDF.
This value can of of three types: floating (no timezone), UTC (suffixed with
a Z) or local time with timezone reference (needs a Timezone object
asociated with it.)
should DATE-TIME be a subclass of DATE? 
- I think so (a specialization)
XML Schema datatypes defines this as well:
dateTime represents a specific instant of time. The ·value space· of dateTime is the space of Combinations of date and time of day values as defined in § 5.4 of [ISO 8601].
-->
<rdfs:subClassOf rdf:resource="&xmlsdt;dateTime" />
<rdfs:subClassOf rdf:resource="#TimeEntry" />
</rdfs:Class>


<rdfs:Class
rdf:ID="DURATION"
 rdfs:label="duration of time"
 rdfs:comment="a duration of time" >

<!-- Again we have a specific syntax associated with this. 
P then
n D (days)
n W (weeks)
[no months or years]

T then
n H (hours)
n M (minutes)
n S (seconds)

see also the DAML work on durations and instants
NOTE: there is also an XMLSchema datatype for duration
-->
</rdfs:Class>



<rdfs:Class
rdf:ID="FLOAT"
 rdfs:label="Float"
 rdfs:comment="float data type" >
<rdfs:subClassOf rdf:resource="&xmlsdt;float" />
</rdfs:Class>


<rdfs:Class
rdf:ID="INTEGER"
 rdfs:label="Integer"
 rdfs:comment="a signed integer" >
<rdfs:subClassOf rdf:resource="&xmlsdt;integer" />
</rdfs:Class>

<rdfs:Class
rdf:ID="PERIOD"
 rdfs:label="a period of time"
 rdfs:comment="a precise period of time. Either a start DATE-TIME and an
end DATE-TIME or a start DATE-TIME and a DURATION" >
<!-- 
I'm not sure how this would look
-->
</rdfs:Class>


<rdfs:Class
rdf:ID="RECUR"
 rdfs:label="Recurrence rule"
 rdfs:comment="A recurrence rule">

<!--Recurrance is hard ;-) I've made a stab at it.

see the properties
#FREQ
#COUNT
#UNTIL
#INTERVAL
#BYSECOND
#BYMINUTE
#BYHOUR
#BYMONTHDAY
#BYYEARDAY
#BYWEEKNO
#BYMONTH
#BYSETPOS
#WKSET
-->

<!--MHA: I think these properties should subclass from RECUR-PROPERTY or some 
such, so it is easy to distinguish these.  Furthermore, we could make RECUR 
the domain of RECUR-PROPERTY. --> 

</rdfs:Class>


<rdfs:Class
rdf:ID="TEXT"
 rdfs:label="Text"
 rdfs:comment="An object with an rdf:value of human-readable text">
<rdfs:subClassOf rdf:resource="&xmlsdt;string"/>

<!--

I think this has to be the case unless rdf:literal is redefined as a
subclass of rdf:resource, because iCalendar RFC 2445 attatches lots of
properties to TEXT. But it might not be the simplest solution in the
future.

-->
</rdfs:Class>


<rdfs:Class
rdf:ID="TIME"
 rdfs:label="Time"
 rdfs:comment="Time of day. Three forms are possible: hour, min, sec
floating, UTC (suffixed by a Z character) and local time with Time zone
reference.">
<!-- ?? and... what is the relationship of DATE and TIME to DATE-TIME and
to each other?-->
<!--from xml schema datatypes time-->
<rdfs:subClassOf rdf:resource="&xmlsdt;time" />
</rdfs:Class>



<rdfs:Class rdf:ID="URI"
 rdfs:label="Uri"
 rdfs:comment="A uri as defined by RFC 1738, RFC 2111 and any other IETF
 registered value format" >
 <!-- do we even need to subclass resource? -->
 <!--MHA: URI is defined in XMLSchema#anyURI.  We can subClass that. 
 -->

 <rdfs:subClassOf rdf:resource="&xmlsdt;anyURI" />
</rdfs:Class>

<rdfs:Class rdf:ID="UTC-OFFSET"
 rdfs:label="UTC offset"
 rdfs:comment="This appears to be a special kind of integer in the iCalendar
 specification." >
 <rdfs:subClassOf rdf:resource="#INTEGER"/>
</rdfs:Class>

<!--Components-->

<rdfs:Class
rdf:ID="VCALENDAR"
 rdfs:label="Calendar"
 rdfs:comment="A calendar of events"/>

<rdfs:Class
rdf:ID="REC-CAL-COMPONENT"
 rdfs:label="Recurring calendar component"
 rdfs:comment="A recurring calendar component. Only VEVENTs, VTODOs and
VJOURNALs can recur" />

<rdfs:Class
rdf:ID="CAL-COMPONENT"
 rdfs:label="Calendar component"
 rdfs:comment="A superclass of all calendar components" />


<rdfs:Class
rdf:ID="VEVENT"
 rdfs:label="Event"
 rdfs:comment="An event">
<rdfs:subClassOf rdf:resource="#CAL-COMPONENT"/>
</rdfs:Class>

<rdfs:Class
rdf:ID="REC-VEVENT"
 rdfs:label="Recurring Event"
 rdfs:comment="A recurring event">
 <rdfs:subClassOf rdf:resource="#VEVENT"/>
 <rdfs:subClassOf rdf:resource="#REC-CAL-COMPONENT"/>
</rdfs:Class>

<rdfs:Class
rdf:ID="ANNIVERSARY"
 rdfs:label="Anniversary"
 rdfs:comment="An event which may occur repeatedly">

<!-- 

I'm not completely sure about this one. If VEVENT is used in this way, it
must have a DATE rather than a DATE-TIME for the DTSTART property. It seems
rather confusing to overload the semantics of DATE-START in this way -
sometimes means the start of a repeating event; sometimes of an actual
event. Plus there is all the recurrance rules stuff as well.

 -->
<rdfs:subClassOf rdf:resource="#REC-VEVENT" />
</rdfs:Class>



<rdfs:Class rdf:ID="VTODO"
 rdfs:label="Todo"
 rdfs:comment="A todo object">
<rdfs:subClassOf rdf:resource="#CAL-COMPONENT" />
</rdfs:Class>


<rdfs:Class
 rdf:ID="REC-VTODO"
 rdfs:label="Recurring TODO"
 rdfs:comment="A recurring todo">
 <rdfs:subClassOf rdf:resource="#VTODO" />
 <rdfs:subClassOf rdf:resource="#REC-CAL-COMPONENT"/>
</rdfs:Class>

<rdfs:Class rdf:ID="VJOURNAL"
 rdfs:label="Journal"
 rdfs:comment="A journal object">
 <rdfs:subClassOf rdf:resource="#CAL-COMPONENT" />
</rdfs:Class>

<rdfs:Class
 rdf:ID="REC-VJOURNAL"
 rdfs:label="Recurring Journal"
 rdfs:comment="A recurring journal entry">
 <rdfs:subClassOf rdf:resource="#VJOURNAL" />
 <rdfs:subClassOf rdf:resource="#REC-CAL-COMPONENT" />
</rdfs:Class>


<rdfs:Class
 rdf:ID="VFREEBUSY"
 rdfs:label="Free-busy"
 rdfs:comment="A free-busy object">
<rdfs:subClassOf rdf:resource="#CAL-COMPONENT"/>
</rdfs:Class>

<rdfs:Class
 rdf:ID="REC-VFREEBUSY"
 rdfs:label="Recurring Free-busy"
 rdfs:comment="A recurring free-busy object">
 <rdfs:subClassOf rdf:resource="#VFREEBUSY" />
 <rdfs:subClassOf rdf:resource="#REC-CAL-COMPONENT"/>
</rdfs:Class>

<!-- VTIMEZONE and VALARM are quite different objects to the other calendar
components. So although RFC 2445 regards them as calendar components, I
don't make them subclasses of CAL-COMPONENT -->

<!--MHA: I agree, they are not like the others-->


<rdfs:Class
rdf:ID="VTIMEZONE"
 rdfs:label="Time zone"
 rdfs:comment="A time zone object" />

<rdfs:Class
 rdf:ID="VALARM"
 rdfs:label="Alarm"
 rdfs:comment="An alarm object" />

<rdfs:Class
 rdf:ID="EMAIL-VALARM"
 rdfs:label="E-Mail alarm"
 rdfs:comment="An alarm that causes an e-mail to be sent to the attendee">
 <rdfs:subClassOf rdf:resource="#VALARM"/>
</rdfs:Class>

<!--Properties-->

<rdfs:Class rdf:ID="Property"
	rdfs:label="iCalendar property"
	rdfs:comment="iCalendar properties derive from this.">
	<rdfs:subClassOf rdf:resource="&rdf;Property"/> 
</rdfs:Class>

<!-- general calendar properties -->

<iCalendar:Property
 rdf:ID="CALSCALE"
 rdfs:label="Calendar scale" 
 rdfs:comment="The calendar scale used for the calendar information in a
VCALENDAR. The default is GREGORIAN.">
<rdfs:domain rdf:resource="#VCALENDAR" /> 
<rdfs:range rdf:resource="http://www.w3.org/2000/01/rdf-schema#Literal" />
<!-- possibly a better domain - UML heirarchy? text? -->
</iCalendar:Property>


<iCalendar:Property
	rdf:ID="METHOD"
 	rdfs:label="Method" 
 	rdfs:comment="See the iTIP RFC for more information about methods">
	<rdfs:domain rdf:resource="#VCALENDAR" /> 
	<rdfs:range rdf:resource="#TEXT" />
</iCalendar:Property>


<iCalendar:Property
	rdf:ID="PRODID"
 	rdfs:label="Product Identifier" 
 	rdfs:comment="The identifier for the product that created the iCalendar
	object">
	<rdfs:domain rdf:resource="#VCALENDAR" /> 
	<rdfs:range rdf:resource="#TEXT" />
<!-- Possibly a resource -->
</iCalendar:Property>


<iCalendar:Property
	rdf:ID="VERSION"
 	rdfs:label="Version of iCalendar spcecification" 
 	rdfs:comment="The higest version number or the minimum and maximum 
	range of the icalendar specification that is needed to interpret the 
	iCalendar object">
<!--not sure how to handle the max/min point - maybe an object? -->
	<rdfs:domain rdf:resource="#VCALENDAR" /> 
	<rdfs:range rdf:resource="#TEXT" />
</iCalendar:Property>


<!-- Component properties -->


<iCalendar:Property
	rdf:ID="ATTACH"
	rdfs:label="Attachment" 
	rdfs:comment="A property pointing to the URI of an attatchment, or an
	object with a BINARY value to point to an inline binary object">
	<rdfs:domain rdf:resource="#CAL-COMPONENT"/> 
	<rdfs:domain rdf:resource="#VALARM" /> 
	<rdfs:range rdf:resource="#Attachment" /> 
</iCalendar:Property>

<!-- An attachement can be binary or URI-->

<rdfs:Class rdf:ID="Attachment"/>
 

<rdfs:Class
	rdf:ID="BINARY-Attachment"
	rdfs:label="Binary Attachment"
	rdfs:comment="A binary-attachment">
	<rdfs:subClassOf rdf:resource="#Attachment"/>
<!-- Correction -->	
<!--	<rdfs:domain rdf:resource="#BINARY"/> -->
<!-- A class cannot have rdfs:domain -->
</rdfs:Class>

<rdfs:Class
	rdf:ID="URI-Attachment"
	rdfs:label="URI Attachemnt"
	rdfs:comment="A URI-attachment">
	<rdfs:subClassOf rdf:resource="#Attachment"/>
<!--Correction -->	
<!--	<rdfs:domain rdf:resource="#URI"/> -->
<!--A class cannot have rdfs:domain -->
</rdfs:Class>

<iCalendar:Property
	rdf:ID="CATEGORIES"
	rdfs:label="Categories" 
	rdfs:comment="Subject categories for the CAL-COMPONENT">
<!-- 
LM: There are several ways to go with this. Either a bag of literals
(TEXTs) or separate literals, or (and this is my prefered option) separate
resources with rdf:values as in DC in RDF. I'm going with the separate
literals (even though TEXT is a resource it is a very constrainted type)
option here.
-->
	<rdfs:domain rdf:resource="#CAL-COMPONENT"/> 
	<rdfs:range rdf:resource="#TEXT" /> 
</iCalendar:Property>

<iCalendar:Property
	rdf:ID="CLASSIFICATION"
	rdfs:label="Classification" 
	rdfs:comment="Classification in terms of privacy of the CAL-COMPONENT">
	<rdfs:domain rdf:resource="#CAL-COMPONENT" /> 
	<rdfs:range rdf:resource="#CLASSIFICATION-CHOICE" />
</iCalendar:Property>

<rdfs:Class rdf:ID="CLASSIFICATION-CHOICE"/>

<!-- 
The options are 
PUBLIC
PRIVATE
CONFDENTIAL
-->

<iCalendar:CLASSIFICATION-CHOICE rdf:ID="PUBLIC"/>
<iCalendar:CLASSIFICATION-CHOICE rdf:ID="PRIVATE"/>
<iCalendar:CLASSIFICATION-CHOICE rdf:ID="CONFIDENTIAL"/>


<iCalendar:Property
	rdf:ID="DESCRIPTION"
	rdfs:label="Description" 
	rdfs:comment="A textual description of the CAL-COMPONENT, more complex
	than that provided by the SUMMARY property">
	<rdfs:domain rdf:resource="#CAL-COMPONENT"/> 
	<rdfs:range rdf:resource="#TEXT" /> 
</iCalendar:Property>

<!--LM: Geographical and location properties. My inclination is to create a
location object, which can a precise longitude and latitude properties and a
textual description. But I haven't done that here. Also - why not
JOURNAL? -->

<!--MHA:   The above idea is ok, I think.  I've implemented it.-->


<iCalendar:Property
 rdf:ID="LOCATION"
 rdfs:label="Location" 
 rdfs:comment="This Location can have a Geographical location applied to it.  
 Otherwise, it is simply a textual description of the location of an EVENT or 
 TODO.">
        <rdfs:domain rdf:resource="#VEVENT" /> 
 	<rdfs:domain rdf:resource="#VTODO" /> 
 	<rdfs:range rdf:resource="#TEXT" /> 
</iCalendar:Property>

<!-- GEO seems ito be missing. added 2001-07-16 by libby -->


<rdfs:Class rdf:ID="GEO"
 rdfs:label="Geographical position"
 rdfs:comment="A geographical location. May have a TEXT description and/or
long/lat properties">
 <rdfs:subClassOf rdf:resource="&xmlsdt;base64binary" />
</rdfs:Class>


<!-- added 2001-07-16 by libby. Could maybe use CN or similar instead of
being so specific -->


<rdf:Property
 rdf:ID="GEO-NAME"
 rdfs:label="Geographical location name"
 rdfs:comment="Geographical location name">
 <rdfs:domain rdf:resource="#GEO"/>
 <rdfs:range rdf:resource="#TEXT" />
</rdf:Property>


<!-- changed LOCATIONs to GEOs as domains  2001-07-16 libby -->


<rdf:Property
 rdf:ID="LONGITUDE"
 rdfs:label="Longitude"
 rdfs:comment="The longitude must be between 0 and 180">
 <rdfs:domain rdf:resource="#GEO"/>
 <rdfs:range rdf:resource="#FLOAT" />
</rdf:Property>

<rdf:Property
 rdf:ID="LATITUDE"
 rdfs:label="Latitude"
 rdfs:comment="The latitude must be between 0 and 90">
 <rdfs:domain rdf:resource="#GEO"/>
 <rdfs:range rdf:resource="#FLOAT" />
</rdf:Property>

<!-- end of location properties -->


<iCalendar:Property
	rdf:ID="PERCENT-COMPLETE"
 	rdfs:label="Percent complete" 
 	rdfs:comment="This property is used by an assignee or delegatee of a 
	VTODO to convey the percent completion of a VTODO to the ORGANIZER">
	<rdfs:domain rdf:resource="#VTODO" /> 
	<rdfs:domain rdf:resource="#VEVENT" /> 
	<rdfs:range rdf:resource="#INTEGER" />
	<!-- ignoring the sign of the INTEGER, presumably -->
</iCalendar:Property>


<iCalendar:Property
	rdf:ID="PRIORITY"
 	rdfs:label="Priority" 
 	rdfs:comment="Defines the relative priority for a calendar component
	(VEVENT or VTODO)">
	<rdfs:domain rdf:resource="#VTODO" /> 
	<rdfs:domain rdf:resource="#VEVENT" /> 
	<rdfs:range rdf:resource="#INTEGER" />
	<!-- ignoring the sign of the INTEGER, presumably -->
</iCalendar:Property>


<iCalendar:Property
	rdf:ID="RESOURCES"
 	rdfs:label="Resources" 
 	rdfs:comment="The equipment or resources anticipated for an activity
	specified by a calendar entity">
<!-- 
Similar considerations apply here as with the CATEGORIES: i.e. bag or
separate, literals or resources. This should probably be resources in
either case, because institutions will need to assign internal identifiers
to resources. Here I have used literals (i.e. the constrained resource
type TEXT), in keeping with the RFC 2445.
This could possibly be extended to encompass ABC-style inputs to a meeting
(including documents for example). Outputs would also be useful. 
-->
 	<rdfs:domain rdf:resource="#CAL-COMPONENT"/> 
	<rdfs:range rdf:resource="#TEXT" /> 
</iCalendar:Property>


<iCalendar:Property
	rdf:ID="STATUS"
 	rdfs:label="Status" 
 	rdfs:comment="The overall status or confirmation for the calendar
	component, used by the ORGANIZER to indicate whether an event is
	(definitely) aking place."> 
<!-- 
possible values for VEVENT are:
TENTATIVE
CONFIRMED
CANCELLED
possible values for VTODO are:
NEEDS-ACTION
COMPLETED
IN-PROCESS
CANCELLED
possible values for VJOURNAL are:
DRAFT
FINAL
CANCELLED
possibly a literal would be more appropriate
MHA: This should probably be a set of choices like CLASSIFICATION
Since the choices are different, this should be subclassed, probably.
-->
</iCalendar:Property>

<iCalendar:Property
	rdf:ID="VEVENT-STATUS"
 	rdfs:label="Event Status" 
 	rdfs:comment="The overall status or confirmation for the event, 
	used by the ORGANIZER to indicate whether an event is
	(definitely) aking place."> 
	<rdfs:domain rdf:resource="#VEVENT"/> 
	<rdfs:range rdf:resource="#VEVENT-STATUS-CHOICE" />
<!-- Correction: Since STATUS has been defined as a Property, the
subPropertyOf should be used -->
<!--	<rdfs:subClassOf rdf:resource="#STATUS"/> -->
	<rdfs:subPropertyOf rdf:resource="#STATUS"/>
</iCalendar:Property>

<rdfs:Class rdf:ID="VEVENT-STATUS-CHOICE"/>

<!--possible values for VEVENT are:-->
<iCalendar:VEVENT-STATUS-CHOICE rdf:ID="TENTATIVE"/>
<iCalendar:VEVENT-STATUS-CHOICE rdf:ID="CONFIRMED"/>
<iCalendar:VEVENT-STATUS-CHOICE rdf:ID="CANCELLED">
   <rdf:type rdf:resource="#VTODO-STATUS-CHOICE"/>
   <rdf:type rdf:resource="#VJOURNAL-STATUS-CHOICE"/>
</iCalendar:VEVENT-STATUS-CHOICE>   

<iCalendar:Property
	rdf:ID="VTODO-STATUS"
 	rdfs:label="ToDo Status" 
 	rdfs:comment="The overall status or confirmation for the todo, 
	used by the ORGANIZER to indicate the status of the todo.">
	<rdfs:domain rdf:resource="#VTODO"/> 
	<rdfs:range rdf:resource="#VTODO-STATUS-CHOICE" />
<!-- Correction: Since STATUS has been defined as a Property, the
subPropertyOf should be used -->
<!--	<rdfs:subClassOf rdf:resource="#STATUS"/> -->
	<rdfs:subPropertyOf rdf:resource="#STATUS"/>
</iCalendar:Property>

<rdfs:Class rdf:ID="VTODO-STATUS-CHOICE"/>

<!--possible values for VTODO are:-->
<iCalendar:VTODO-STATUS-CHOICE rdf:ID="NEEDS-ACTION"/>
<iCalendar:VTODO-STATUS-CHOICE rdf:ID="COMPLETED_STATUS"/>
<iCalendar:VTODO-STATUS-CHOICE rdf:ID="IN-PROCESS"/>
<!-- The ID CANCELLED is not unique -->
<!-- Through the mechanism of multiple classification of resources, it was defined above -->
<!-- <iCalendar:VTODO-STATUS-CHOICE rdf:ID="CANCELLED"/> -->


<iCalendar:Property
	rdf:ID="VJOURNAL-STATUS"
 	rdfs:label="Journal Status" 
 	rdfs:comment="The overall status of the Journal entry.">
	<rdfs:domain rdf:resource="#VJOURNAL"/> 
	<rdfs:range rdf:resource="#VJOURNAL-STATUS-CHOICE" />
<!-- Correction: Since STATUS has been defined as a Property, the
subPropertyOf should be used -->
<!--	<rdfs:subClassOf rdf:resource="#STATUS"/> -->
	<rdfs:subPropertyOf rdf:resource="#STATUS"/>
</iCalendar:Property>

<rdfs:Class rdf:ID="VJOURNAL-STATUS-CHOICE"/>

<!--possible values for VJOURNAL are:-->
<iCalendar:VJOURNAL-STATUS-CHOICE rdf:ID="DRAFT"/>
<iCalendar:VJOURNAL-STATUS-CHOICE rdf:ID="FINAL"/>
<!-- The ID CANCELLED is not unique -->
<!-- Through the mechanism of multiple classification of resources, it was defined above -->
<!-- <iCalendar:VJOURNAL-STATUS-CHOICE rdf:ID="CANCELLED"/> -->

<iCalendar:Property
	rdf:ID="SUMMARY"
	rdfs:label="Summary" 
	rdfs:comment="A one-line textual summary of the CAL-COMPONENT or VALARM">
	<rdfs:domain rdf:resource="#CAL-COMPONENT"/> 
	<rdfs:domain rdf:resource="#VALARM" /> 
	<rdfs:range rdf:resource="#TEXT" /> 
</iCalendar:Property>

<!-- Date and time component properties -->

<iCalendar:Property
	rdf:ID="COMPLETED"
	rdfs:label="Completed" 
	rdfs:comment="Defines the date and time that a VTODO was actually completed. The date and time must be in UTC format (i.e suffixed with	a Z)">
	<rdfs:domain rdf:resource="#VTODO" /> 
	<rdfs:range rdf:resource="#DATE-TIME" />
<!--LM: It would be more general to make the domain a DATE rather than a 
DATE-TIME. -->
<!--MHA: Or perhaps a TimeEntry -->
</iCalendar:Property>


<iCalendar:Property
	rdf:ID="DTEND"
	rdfs:label="Date-time end" 
	rdfs:comment="The date and time that the a calendar component ends">
	<rdfs:domain rdf:resource="#VEVENT" /> 
	<rdfs:domain rdf:resource="#VFREEBUSY" /> 
	<rdfs:range rdf:resource="#TimeEntry" />
<!--LM: The default range in RFC 2445 is DATE-TIME, but since we have made
DATE-TIME a subclass of DATE, and the domain can be DATE-TIME or DATE, we
make the range a DATE. -->
<!--MHA: If we subclass DATE and DATE-TIME from TimeEntry, we can
use TimeEntry as the range.-->
</iCalendar:Property>

<iCalendar:Property
	rdf:ID="DUE"
 	rdfs:label="Date time due" 
 	rdfs:comment="Defines the date and time when the VTODO is expected to 
	be completed">
	<rdfs:domain rdf:resource="#VTODO" /> 
	<rdfs:range rdf:resource="#TimeEntry" /> 
<!--LM: The default range in RFC 2445 is DATE-TIME, but since we have made
DATE-TIME a subclass of DATE, and the domain can be DATE-TIME or DATE, we
make the range a DATE. -->
<!--MHA: If we subclass DATE and DATE-TIME from TimeEntry, we can
use TimeEntry as the range.-->
</iCalendar:Property>


<iCalendar:Property
	rdf:ID="DTSTART"
	rdfs:label="Date time start" 
 	rdfs:comment="Specifies when the calendar component begins. If used 
	with a VFREEBUSY component, the time must be in UTC format">
	<rdfs:domain rdf:resource="#CAL-COMPONENT"/> 
	<rdfs:domain rdf:resource="#VTIMEZONE" /> 
	<rdfs:range rdf:resource="#DATE" /> 
<!--LM: The default range in RFC 2445 is DATE-TIME, but since we have made
DATE-TIME a subclass of DATE, and the domain can be DATE-TIME or DATE, we
make the range a DATE. -->
<!--MHA: If we subclass DATE and DATE-TIME from TimeEntry, we can
use TimeEntry as the range.-->
</iCalendar:Property>

<!-- For DURATION also see the DAML-S work (also instant) -->
<!-- Also, there is a DURATION datatype in the XML Schema -->

<iCalendar:Property
	rdf:ID="DURATION-PROP"
	rdfs:label="Duration" 
	rdfs:comment="A positive duration of time">
	<rdfs:domain rdf:resource="#CAL-COMPONENT"/> 
	<rdfs:domain rdf:resource="#VALARM" /> 
	<rdfs:range rdf:resource="#DURATION" />
</iCalendar:Property>


<iCalendar:Property
	rdf:ID="FREEBUSY-PROP"
	rdfs:label="Free-busy time" 
	rdfs:comment="Defines one or more free or busy time intervals. the
	duration times and dates must be in UTC format">
	<rdfs:domain rdf:resource="#VFREEBUSY" /> 
	<rdfs:range rdf:resource="#PERIOD" /> 
</iCalendar:Property>


<iCalendar:Property
 rdf:ID="TRANSP"
 rdfs:label="Time transparency" 
 rdfs:comment="Defines whether an event is transparent or not to busy 
 time searches. VJOURNALs, for example, are always transparent, as are 
 VTODOS. VEVENTS can be made so."> 
<!--
TRANSPARENT
OPAQUE
possibly a literal would be more appropriate
MHA: Perhaps a choice - see Classification above
-->
 <rdfs:domain rdf:resource="#VEVENT" /> 
 <rdfs:range rdf:resource="#TRANSP-CHOICE" />
</iCalendar:Property>

<rdfs:Class rdf:ID="TRANSP-CHOICE"/>

<iCalendar:TRANSP-CHOICE rdf:ID="TRANSPARENT"/>
<iCalendar:TRANSP-CHOICE rdf:ID="OPAQUE"/>


<!-- Time zone component properties -->


<iCalendar:Property
 rdf:ID="TZID"
 rdfs:label="Time zone identifier" 
 rdfs:comment="Specifies the identifier (TEXT in the RFC 2445) that uniquely
 identifies the VTIMEZONE calendar component. It must be specified in a
 VTIMEZONE component">
 <!-- 
 I've made this a resource rather than TEXT 
 Could it also be specified on other objects??
 -->
 <rdfs:domain rdf:resource="#VTIMEZONE" />
 <rdfs:range rdf:resource="http://www.w3.org/2000/01/rdf-schema#Resource" />
</iCalendar:Property>


<iCalendar:Property
 rdf:ID="TZNAME"
 rdfs:label="Time zone name" 
 rdfs:comment="The customary designation for a time zone description. you
 can also have a language tag on this, which indicates that TEXT
 should be a subclass of resource, not literal (this is what I have done)">
 <rdfs:domain rdf:resource="#VTIMEZONE" />
 <rdfs:range rdf:resource="#TEXT" /> 
</iCalendar:Property>



<iCalendar:Property
rdf:ID="TZOFFSETFROM"
 rdfs:label="Time zone offset from" 
 rdfs:comment="Specifies the offset which is in use prior to this time zone
observance. Must be specified in a VTIMEZONE calendar component">
<rdfs:domain rdf:resource="#VTIMEZONE" />
<rdfs:range rdf:resource="#UTC-OFFSET" />
</iCalendar:Property>


<iCalendar:Property
rdf:ID="TZOFFSETTO"
 rdfs:label="Time zone offset to" 
 rdfs:comment="Specifies the offset which is in this time zone
observance. Must be specified in a VTIMEZONE calendar component">
<rdfs:domain rdf:resource="#VTIMEZONE" />
<rdfs:range rdf:resource="#UTC-OFFSET" />
</iCalendar:Property>


<iCalendar:Property
 rdf:ID="TZURL"
 rdfs:label="Time zone url" 
 rdfs:comment="Points to a network resource which a VTIMEZONE can point to
 to get an up-to-date versioon of itself. It can be specified in a VTIMEZONE
 calendar component">
 <rdfs:domain rdf:resource="#VTIMEZONE" />
 <rdfs:range rdf:resource="#URI" />
</iCalendar:Property>


<!-- relationship component properties -->

<!-- see also property parameters -->

<iCalendar:Property
 rdf:ID="ATTENDEE"
 rdfs:label="Attendee" 
 rdfs:comment="Defines an attendee within a calendar component">
 <rdfs:domain rdf:resource="#CAL-COMPONENT"/> 
 <rdfs:domain rdf:resource="#EMAIL-VALARM"/>
 <rdfs:range rdf:resource="#CAL-ADDRESS"/> 
</iCalendar:Property>



<iCalendar:Property
 rdf:ID="CONTACT"
 rdfs:label="Contact" 
 rdfs:comment="A representation or a reference to contact information
 associated with a calendar component">
 <rdfs:domain rdf:resource="#CAL-COMPONENT"/> 
 <rdfs:range rdf:resource="#TEXT"/> 
<!-- 
LM: This is a very confusing one. Contact information would be better attatched
to a CAL-USER or other agent. Presumably the contact for a given event is
the organizer? 

Note that a calendar address should be an object not just an address.
-->

<!--
MHA: I believe that TEXT will do here, with an altrepparam of a URI 
available if needed.
Incidentally, this could be the organizer or some other contact person (such
as if the organizer is out of town?).  I think it's like reply-to wrt email.
-->
</iCalendar:Property>


<iCalendar:Property
 rdf:ID="ORGANIZER"
 rdfs:label="Organizer" 
 rdfs:comment="Points to the organizer of the calendar component">
 <rdfs:domain rdf:resource="#CAL-COMPONENT"/> 
 <rdfs:range rdf:resource="#CAL-ADDRESS"/> 
 <!--
 Note that a calendar address should be an object not just an address.
 -->
</iCalendar:Property>


<iCalendar:Property
 rdf:ID="RECURRANCE-ID"
 rdfs:label="Recurrance identifier" 
 rdfs:comment="An identifier for a specific instance of a REC-CAL-COMPONENT 
 (a VEVENT, VTODO or VJOURNAL)">
 <rdfs:domain rdf:resource="#REC-CAL-COMPONENT"/> 
 <rdfs:range rdf:resource="#TimeEntry" />
 <!--
 LM: DATE is used as the superclass of DATE-TIME.
 MHA: I changed it to be a TimeEntry, which is the superclass of DATE and DATE-
      TIME in this schema.

 LM: The RFC 2445 says that RECURRANCE-ID should be the DTSTART of the
 REC-CAL-COMPONENT, i.e. the date the repetitions started, NOT the date and
 time of instances of the REC-CAL-COMPONENT starting. I think this is
 confusing, subject to becoming unlinked with the DTSTART value (which can
 change through exceptions) and non-globally unique.
 see also #RANGE
 -->
</iCalendar:Property>

<rdf:Property
 rdf:ID="RELATED-TO"
 rdfs:label="Related to" 
 rdfs:comment="A relationship or reference between one calendar component
 and another">
 <rdfs:domain rdf:resource="#CAL-COMPONENT" /> 
 <rdfs:range rdf:resource="&rdfs;Resource" />
 <!--
 LM: RELATED-TO has to be a class unless we make the RELTYPE values 
 subproperties of RELTYPE. I think this is what we would have to do. It could 
 be useful for specifying the details of a meeting or track at a conference in  greater detail.
 MHA: Not sure about this.  For now, I've made it rdf;Resource, so it 
 encompasses all components.
 -->
</rdf:Property>

<!--
 MHA: URL used to have a domain of VCALENDAR, which seems wrong.  I've made it 
      CAL-COMPONENT 
-->


<rdf:Property
 rdf:ID="URL"
 rdfs:label="URL" 
 rdfs:comment="Points to a URL at whihc this calendar information may be
 found, for example a more recent version">
 <rdfs:domain rdf:resource="#CAL-COMPONENT" />
 <rdfs:range rdf:resource="#URI" />
</rdf:Property>



<rdf:Property
 rdf:ID="UID"
 rdfs:label="Unique identifier" 
 rdfs:comment="The globally unique identifier for the calendar component">
 <rdfs:domain rdf:resource="#CAL-COMPONENT" />
 <rdfs:range rdf:resource="&rdfs;Resource" />
 <!-- in RFC 2445 the range is a TEXT object, but it should definitely be a 
 resource --> 
</rdf:Property>


<!-- recurrance component properties -->

<rdf:Property
 rdf:ID="EXDATE"
 rdfs:label="Recurrance Date exceptions" 
 rdfs:comment="Defines the list of date/time exceptions for a recurring
 calendar component">
 <rdfs:domain rdf:resource="#REC-CAL-COMPONENT" /> 
 <rdfs:range rdf:resource="#TimeEntry" /> 
 <!--
 LM: Using Date as superclass of DATE-TIME.
 MHA: I changed this to TimeEntry. (Superclass of DATE and DATE-TIME)
 This might be better as a bag
 -->
</rdf:Property>

<rdf:Property
 rdf:ID="EXRULE"
 rdfs:label="Recurrance exception rule" 
 rdfs:comment="Points to a rule or repeating pattern for an exception to a
 recurrance set">
 <rdfs:domain rdf:resource="#REC-CAL-COMPONENT"/> 
 <rdfs:range rdf:resource="#RECUR" />
</rdf:Property>


<rdf:Property
 rdf:ID="RDATE"
 rdfs:label="Recurrance date" 
 rdfs:comment="Defines the list of dates/times for a recurring
 calendar component">
 <rdfs:domain rdf:resource="#REC-CAL-COMPONENT" /> 
 <rdfs:range rdf:resource="#TimeEntry" /> 
 <!--
 LM: Using Date as superclass of DATE-TIME.
 MHA: Changed it to TimeEntry
 This might be better as a bag
 -->
</rdf:Property>



<rdf:Property
 rdf:ID="RRULE"
 rdfs:label="Recurrance rule" 
 rdfs:comment="Points to a rule or repeating pattern for an exception to a
 recurrance set">
 <rdfs:domain rdf:resource="#REC-CAL-COMPONENT" /> 
 <rdfs:range rdf:resource="#RECUR" />
</rdf:Property>


<!-- recurrance properties

#FREQ
#COUNT
#UNTIL
#INTERVAL
#BYSECOND
#BYMINUTE
#BYHOUR
#BYMONTHDAY
#BYYEARDAY
#BYWEEKNO
#BYMONTH
#BYSETPOS
#WKSET

-->




<rdf:Property rdf:ID="FREQ"
 rdfs:label="Frequency" 
 rdfs:comment="The type of the recurrance rule">
 <rdfs:domain rdf:resource="#RECUR" />
 <rdfs:range rdf:resource="#TEXT" />
<!--
SECONDLY
MINUTELY
HOURLY
DAILY
WEEKLY
MONTHLY
YEARLY
possibly should be a literal
MHA: or some kind of choice.
-->
</rdf:Property>


<rdf:Property rdf:ID="INTERVAL"
 rdfs:label="Interval" 
 rdfs:comment="How often the recurrance rule repeats. The dfault is 1,
i.e. _every_ year etc">
<rdfs:domain rdf:resource="#RECUR" />
<rdfs:range rdf:resource="#INTEGER" />
<!-- INTEGER sign ignored -->
</rdf:Property>



<rdf:Property rdf:ID="UNTIL"
 rdfs:label="Until" 
 rdfs:comment="Defines a date-time value which bounds the recurrance rule in
an inclusive manner. If a DATE, must be UTC">
<rdfs:domain rdf:resource="#RECUR" />
<rdfs:range rdf:resource="#TimeEntry" />
<!--
LM: Date used as superclass of DATE-TIME
MHA: Changed to TimeEntry
-->
</rdf:Property>


<rdf:Property
rdf:ID="COUNT"
 rdfs:label="Count" 
 rdfs:comment="the number of occurrances at which to range-bound the
recurance. If specified, the DTSTART value counts as the first of these">
<rdfs:domain rdf:resource="#RECUR" />
<rdfs:range rdf:resource="#INTEGER" />
<!-- INTEGER sign ignored -->
</rdf:Property>


<rdf:Property rdf:ID="BYSECOND"
 rdfs:label="By second" 
 rdfs:comment="A list of second values for recurrance">
<rdfs:domain rdf:resource="#RECUR" />
<rdfs:range rdf:resource="#INTEGER" />
<!-- INTEGER sign ignored 0-59 only. maybe should be a bag -->
</rdf:Property>


<rdf:Property rdf:ID="BYMINUTE"
 rdfs:label="By minute" 
 rdfs:comment="A list of minute values for recurrance">
<rdfs:domain rdf:resource="#RECUR" />
<rdfs:range rdf:resource="#INTEGER" />
<!-- INTEGER sign ignored 0-59 only. maybe should be a bag -->
</rdf:Property>


<rdf:Property
rdf:ID="BYHOUR"
 rdfs:label="By hour" 
 rdfs:comment="A list of hour values for recurrance">
<rdfs:domain rdf:resource="#RECUR" />
<rdfs:range rdf:resource="#INTEGER" />
<!-- INTEGER sign ignored 0-23 only. maybe should be a bag -->
</rdf:Property>



<rdf:Property rdf:ID="BYDAY"
 rdfs:label="By day" 
 rdfs:comment="A list of day values for recurrance">
<rdfs:domain rdf:resource="#RECUR" />
<rdfs:range rdf:resource="#TEXT" />

<!-- 
MO
TU
WE
TH
FR
SA
SU
It can also be prefixed by a positive or negative integer representing the
nth occurance of the day from the beginning or end of the month.
So this is looking like a day object or a day of the month object.
Maybe should be literals, maybe should be a bag 
MHA: maybe should be choices
-->
</rdf:Property>


<rdf:Property rdf:ID="BYMONTHDAY"
 rdfs:label="By month day" 
 rdfs:comment="A list of INTEGERS representing days in a month values for
recurrance">
<rdfs:domain rdf:resource="#RECUR" />
<rdfs:range rdf:resource="#INTEGER" />
<!-- INTEGER sign represents from the beginning/end of the month.
 0-31 only. Maybe should be a bag -->
</rdf:Property>



<rdf:Property rdf:ID="BYYEARDAY"
 rdfs:label="By year day" 
 rdfs:comment="A list of INTEGERS representing days in a year values for
recurrance">
<rdfs:domain rdf:resource="#RECUR" />
<rdfs:range rdf:resource="#INTEGER" />
<!-- INTEGER sign represents from the beginning/end of the year.
 0-366 only. Maybe should be a bag -->
</rdf:Property>


<rdf:Property rdf:ID="BYWEEKNO"
 rdfs:label="By week number" 
 rdfs:comment="A list of INTEGERS representing weeks in a year values for
recurrance">
<rdfs:domain rdf:resource="#RECUR" />
<rdfs:range rdf:resource="#INTEGER" />
<!-- INTEGER sign represents from the beginning/end of the year.
 0-53 only. Maybe should be a bag -->
</rdf:Property>



<rdf:Property rdf:ID="BYMONTH"
 rdfs:label="By month" 
 rdfs:comment="A list of INTEGERS representing months in a year values for
recurrance">
<rdfs:domain rdf:resource="#RECUR" />
<rdfs:range rdf:resource="#INTEGER" />
<!-- INTEGER sign represents from the beginning/end of the year.
 0-12 only. Maybe should be a bag -->
</rdf:Property>



<rdf:Property rdf:ID="WKST"
 rdfs:label="Working week start" 
 rdfs:comment="Specifies the day on which the working week starts">
<!-- 
MO
TU
WE
TH
FR
SA
SU
MHA: Should probably be choices.
-->
<rdfs:domain rdf:resource="#RECUR" />
<rdfs:range rdf:resource="#TEXT" />
<!-- 
maybe should be a literal; maybe a bag
-->
</rdf:Property>



<rdf:Property rdf:ID="BYSETPOS"
 rdfs:label="By set position" 
 rdfs:comment="A list of INTEGERS representing the nth occurrance of the
repetition within the set of evets specified by the rule">
<rdfs:domain rdf:resource="#RECUR" />
<rdfs:range rdf:resource="#INTEGER" />
<!-- INTEGER sign represents from the beginning/end of the set.
Maybe should be a bag -->
</rdf:Property>


<!-- Alarm component properties -->



<rdf:Property rdf:ID="ACTION"
 rdfs:label="Action" 
 rdfs:comment="The action to be invoked when the alarm is triggered. Must
be specified once in a VALARM">
<rdfs:domain rdf:resource="#VALARM" />
<rdfs:range rdf:resource="#TEXT" />
<!-- 
AUDIO
DISPLAY
EMAIL
PROCEEDURE
LM: maybe should be literal

MHA: Actually, this is a bit more complicated since each action 
denotes a different kind of alarm, really.  Perhaps it should be 
folded into subclasses of VALARM?
-->
</rdf:Property>



<rdf:Property rdf:ID="REPEAT"
 rdfs:label="Repeat Count" 
 rdfs:comment="The number of times the alarm should be repeated after the
initial trigger">
<rdfs:domain rdf:resource="#VALARM" />
<rdfs:range rdf:resource="#INTEGER" />
<!-- 
sign ignored
-->
</rdf:Property>


<iCalendar:Property rdf:ID="TRIGGER"
 rdfs:label="Trigger" 
 rdfs:comment="When an alarm is triggered">
<rdfs:domain rdf:resource="#VALARM" />
<!-- 
LM: but range can also be a DATE-TIME (UTC). The relationship between these
needs more specification. The duration is used because it is the positive or
negative distance in time from the beginning or end of the event.
see also #RELATED
MHA: Ok, how about we subclass the TRIGGER (REL-TRIGGER and ABS-TRIGGER), 
since they have different parameters.
-->
</iCalendar:Property>

<iCalendar:Property rdf:ID="REL-TRIGGER"
 rdfs:label="Relative Trigger"
 rdfs:comment="When an alarm is triggered -- relative to the associated event
 or todo">
 <!-- Correction: Since TRIGGER has been defined as a Property, the
subPropertyOf should be used -->
<!--	<rdfs:subClassOf rdf:resource="#TRIGGER"/> -->
<rdfs:domain rdf:resource="#VALARM" />
 <rdfs:subPropertyOf rdf:resource="#TRIGGER"/>
 <rdfs:range rdf:resource="#DURATION"/>
</iCalendar:Property>

<iCalendar:Property rdf:ID="ABS-TRIGGER"
 rdfs:label="Absolute Trigger"
 rdfs:comment="When an alarm is triggered -- date and time or just date.">
<!-- Correction: Since TRIGGER has been defined as a Property, the
subPropertyOf should be used -->
<!--	<rdfs:subClassOf rdf:resource="#TRIGGER"/> -->
 <rdfs:subPropertyOf rdf:resource="#TRIGGER"/>
<rdfs:domain rdf:resource="#VALARM" />
<rdfs:range rdf:resource="#TimeEntry"/>
</iCalendar:Property>



<!-- change management component properties -->



<iCalendar:Property rdf:ID="CREATED"
 rdfs:label="Date/time created" 
 rdfs:comment="Date/time a CAL-COMPONENT was created (not VFREEBUSY) (UTC)">
<rdfs:domain rdf:resource="#CAL-COMPONENT" /> 
<rdfs:range rdf:resource="#DATE-TIME" />
</iCalendar:Property>	


<iCalendar:Property rdf:ID="DTSTAMP"
 rdfs:label="Date/time stamp" 
 rdfs:comment="Date/time a VCALENDAR was created (UTC)">
<rdfs:domain rdf:resource="#VCALENDAR" />
<rdfs:range rdf:resource="#DATE-TIME" />
</iCalendar:Property>	


<iCalendar:Property rdf:ID="LAST-MODIFIED"
 rdfs:label="Date/time last modified" 
 rdfs:comment="Date/time a CAL-COMPONENT was last modified (not VFREEBUSY) 
(UTC)">
 <!-- 
 why not VFREEBUSY? 
 -->
 <rdfs:domain rdf:resource="#CAL-COMPONENT"/> 
 <rdfs:domain rdf:resource="#VTIMEZONE" />
 <rdfs:range rdf:resource="#DATE-TIME" />
</iCalendar:Property>	



<iCalendar:Property rdf:ID="SEQUENCE"
 rdfs:label="Sequence" 
 rdfs:comment="The revision number of a calendar component wh=ithin a
 sequence of revisions (not VFREEBUSY)">
 <!--
 starts with ); any time the ORGANIZER makes changes to
 DTSTART
 DTEND
 DUE
 RDATE
 RRULE
 EXDATE
 EXRULEW
 STATUS
 the sequence number must be incremented.
 The ORGANIZER can also force an increment is he thinks that a change made
 may jeopardize attendance
 why not VFREEBUSY?
 -->
 <rdfs:domain rdf:resource="#CAL-COMPONENT"/> 
 <rdfs:range rdf:resource="#INTEGER" />
</iCalendar:Property>	


<!-- Miscellaneous component properties -->

<!-- Non standard properties -->

<!-- These can be applied to all iCal components.  For now,
     I've made the domain resource.  -->

<iCalendar:Property rdf:ID="X-PROP"
 rdfs:label="Non-standard Property"
 rdfs:comment="Any properties that aren't pre-defined.">
 <rdfs:domain rdf:resource="#CAL-COMPONENT"/>
 <rdfs:domain rdf:resource="#VALARM"/>
 <rdfs:domain rdf:resource="#VTIMEZONE"/>
 <rdfs:range rdf:resource="&rdfs;Resource"/> 
</iCalendar:Property>

<!-- Request status -->

<iCalendar:Property rdf:ID="REQUEST-STATUS"
 rdfs:label="Request status" 
 rdfs:comment="The status code for a scheduling request">
<rdfs:domain rdf:resource="#CAL-COMPONENT" /> 
<rdfs:range rdf:resource="#TEXT" />
</iCalendar:Property>	


<!-- iCalendar Parameters-->

<rdfs:Class rdf:ID="Parameter"
 rdfs:label="Property Parameter"
 rdfs:comment="All iCalendar property parameters subclass from this class">
 <rdfs:subClassOf rdf:resource="&rdf;Property"/>
</rdfs:Class>  

<iCalendar:Parameter rdf:ID="ALTREP">
	<rdfs:comment>Alternate Text Representation</rdfs:comment>

<!-- According to the RDF Schema Specification, the value of a domain property
should be a class. However, DESCRIPTION, LOCATION etc are defined as
Properties -->

<!--	<rdfs:domain rdf:resource="#DESCRIPTION"/> -->
<!-- COMMENT has not been defined -->
<!--        <rdfs:domain rdf:resource="#COMMENT"/> -->
<!--	<rdfs:domain rdf:resource="#LOCATION"/> -->
<!--	<rdfs:domain rdf:resource="#RESOURCES"/> -->
<!--	<rdfs:domain rdf:resource="#SUMMARY"/> -->
<!--	<rdfs:domain rdf:resource="#CONTACT"/> -->
        <rdfs:range rdf:resource="#URI"/>
</iCalendar:Parameter>

<iCalendar:Parameter rdf:ID="CN">
	<rdfs:comment>Common Name</rdfs:comment>
<!--	<rdfs:domain rdf:resource="#ATTENDEE"/> -->
<!--	<rdfs:domain rdf:resource="#ORGANIZER"/> -->
	<rdfs:range rdf:resource="&rdfs;Literal"/>
</iCalendar:Parameter>

<iCalendar:Parameter rdf:ID="CUTYPE">
	<rdfs:comment>Calendar User Type</rdfs:comment>
<!--	<rdfs:domain rdf:resource="#ATTENDEE"/> -->
	<rdfs:range rdf:resource="&rdfs;Literal"/>
</iCalendar:Parameter>

<iCalendar:Parameter rdf:ID="DELEGATED-FROM">
	<rdfs:comment>Delegators</rdfs:comment>
<!--	<rdfs:domain rdf:resource="#ATTENDEE"/> -->
	<rdfs:range rdf:resource="#CAL-ADDRESS"/>
</iCalendar:Parameter>

<iCalendar:Parameter rdf:ID="DELEGATED-TO">
	<rdfs:comment>Delegatees</rdfs:comment>
<!--	<rdfs:domain rdf:resource="#ATTENDEE"/> -->
	<rdfs:range rdf:resource="#CAL-ADDRESS"/>
</iCalendar:Parameter>

<iCalendar:Parameter rdf:ID="DIR">
	<rdfs:comment>Directory Entry Reference</rdfs:comment>
<!--	<rdfs:domain rdf:resource="#ATTENDEE"/>
	<rdfs:domain rdf:resource="#ORGANIZER"/> -->
	<rdfs:range rdf:resource="#URI"/>
</iCalendar:Parameter>

<!-- 
 MHA: What does the inline encoding paramter apply to? 
-->

<iCalendar:Parameter rdf:ID="ENCODING">
	<rdfs:comment>Inline Encoding</rdfs:comment>
	<rdfs:range rdf:resource="&rdfs;Resource"/>
</iCalendar:Parameter>

<iCalendar:Parameter rdf:ID="FMTTYPE">
	<rdfs:comment>Format Type</rdfs:comment>
<!--	<rdfs:domain rdf:resource="#ATTACH"/> -->
	<rdfs:range rdf:resource="#TEXT"/>
</iCalendar:Parameter>

<iCalendar:Parameter rdf:ID="FBTYPE">
	<rdfs:comment>Free/Busy Time Type</rdfs:comment>
<!--	<rdfs:domain rdf:resource="#FREEBUSY-PROP"/> -->
	<rdfs:range rdf:resource="#TEXT"/>
</iCalendar:Parameter>

<iCalendar:Parameter rdf:ID="LANGUAGE">
	<rdfs:comment>Language</rdfs:comment>
<!--	<rdfs:domain rdf:resource="#CATEGORIES"/> -->
<!--	<rdfs:domain rdf:resource="#COMMENT"/> -->
<!--	<rdfs:domain rdf:resource="#LOCATION"/> -->
<!--	<rdfs:domain rdf:resource="#RESOURCES"/> -->
<!--	<rdfs:domain rdf:resource="#SUMMARY"/> -->
<!--	<rdfs:domain rdf:resource="#TZNAME"/> -->
<!--	<rdfs:domain rdf:resource="#ATTENDEE"/> -->
<!--	<rdfs:domain rdf:resource="#CONTACT"/> 
	<rdfs:domain rdf:resource="#ORGANIZER"/> -->
<!--        <rdfs:domain rdf:resource="#X-PROP"/> -->
	<rdfs:range rdf:resource="#TEXT"/>
</iCalendar:Parameter>

<iCalendar:Parameter rdf:ID="MEMBER">
	<rdfs:comment>Group or List Membership</rdfs:comment>
<!--	<rdfs:domain rdf:resource="#ATTENDEE"/> -->
	<rdfs:range rdf:resource="#CAL-ADDRESS"/>
</iCalendar:Parameter>

<iCalendar:Parameter rdf:ID="PARTSTAT">
	<rdfs:comment>Participation Status</rdfs:comment>
<!--	<rdfs:domain rdf:resource="#ATTENDEE"/> -->
	<rdfs:range rdf:resource="#TEXT"/>
</iCalendar:Parameter>

<!-- 
 The RANGE should be one of two choices - THISANDPRIOR and THISANDFUTURE.
-->

<rdfs:Class rdf:ID="RANGE-CHOICE"/>

<iCalendar:Parameter rdf:ID="RANGE">
	<rdfs:comment>Recurrence Identifier Range</rdfs:comment>
<!--	<rdfs:domain rdf:resource="#RECURRANCE-ID"/> -->
	<rdfs:range rdf:resource="&rdfs;Literal"/>
</iCalendar:Parameter>

<iCalendar:RANGE-CHOICE rdf:ID="THISANDPRIOR"/>
<iCalendar:RANGE-CHOICE rdf:ID="THISANDFUTURE"/>


<iCalendar:Parameter rdf:ID="RELTYPE">
	<rdfs:comment>Alarm Trigger Relationship</rdfs:comment>
<!--	<rdfs:domain rdf:resource=""/> -->
<!--
PARENT
CHILD
SIBLING
This property means that RELATED-TO has to be a class unless we make the
RELTYPE values subproperties of RELTYPE. I think this is what we would have 
to do. It could be useful for specifying the details of a meeting or track
at a conference in greater detail.
-->
	<rdfs:range rdf:resource="#TEXT"/>
</iCalendar:Parameter>

<!-- another three-way relationship - the role of an attendee in event-->

<iCalendar:Parameter rdf:ID="ROLE">
	<rdfs:comment>Participation Role</rdfs:comment>
<!--	<rdfs:domain rdf:resource="#ATTENDEE"/> -->
	<rdfs:range rdf:resource="#TEXT"/>
</iCalendar:Parameter>
<!--

CHAIR
REQ-PARTICIPANT 
OPT-PARTICIPANT 
NON-PARTICIPANT 

(MHA: and anything else, really.)
-->


<iCalendar:Parameter rdf:ID="RSVP">
	<rdfs:comment>RSVP Expectation</rdfs:comment>
<!--	<rdfs:domain rdf:resource="#ATTENDEE"/> -->
<!-- 
LM: another three-way relationship - the RSVP expectation from the 
cal-user as regards the event

MHA: actually, this and the previous ROLE can only be applied to attendees 
(not organizer, for example)
-->
	<rdfs:range rdf:resource="#BOOLEAN"/>
</iCalendar:Parameter>


<iCalendar:Parameter rdf:ID="SENT-BY">
	<rdfs:comment>Sent By</rdfs:comment>
<!--	<rdfs:domain rdf:resource="#ATTENDEE"/>
	<rdfs:domain rdf:resource="#ORGANIZER"/> -->
	<rdfs:range rdf:resource="#CAL-ADDRESS"/>
</iCalendar:Parameter>

<iCalendar:Parameter rdf:ID="TZID_PARAMETER">
	<rdfs:comment>"Specifies the identifier for the time zone definition.
Uniquely identifies a VTIMEZONE calendar component"</rdfs:comment>
<!-- in RFC 2445 this is a string, but should be aresource -->
<!--	<rdfs:domain rdf:resource="#DTSTART"/> -->
<!--	<rdfs:domain rdf:resource="#DUE"/> -->
<!--	<rdfs:domain rdf:resource="#RECURRANCE-ID"/> -->
<!--	<rdfs:domain rdf:resource="#EXDATE"/>  -->
<!--	<rdfs:domain rdf:resource="#RDATE"/>  -->
	<rdfs:range rdf:resource="&rdfs;Resource"/>
</iCalendar:Parameter>

<iCalendar:Parameter rdf:ID="VALUE">
	<rdfs:comment>Value Data Type</rdfs:comment>
	<rdfs:range rdf:resource="&rdfs;Resource"/>
</iCalendar:Parameter>


</rdf:RDF>
