<?xml version="1.0"?>

<rdf:RDF xml:lang="en"
	 xmlns:rdf="http://www.w3.org/1999/02/22-rdf-syntax-ns#" 
	 xmlns:rdfs="http://www.w3.org/2000/01/rdf-schema#"> 

	<rdfs:Class rdf:ID="LearningObject">
	</rdfs:Class>
	
	<rdfs:Class rdf:ID="Program">
		<rdfs:subClassOf rdf:resource="#LearningObject"/>
		<rdfs:comment>This class is a direct subclass of the LearningObject class. The Program class represents a grouping of courses that lead towards a university degree, i.e. the Computer Science Department of the University of Crete Undergraduate Program, of which the CS252 Course is a part.</rdfs:comment>
	</rdfs:Class>

	<rdfs:Class rdf:ID="Course">
		<rdfs:subClassOf rdf:resource="#LearningObject"/>
		<rdfs:comment>This class is a direct subclass of the LearningObject class. This class represents LOs that consist of more than one modules or lessons that are longer than 10 hours, i.e. the CS252 Course consists of a number of modules, or alternatively, of lessons with more than 10 hours of duration.</rdfs:comment>
	</rdfs:Class>
	
	<rdfs:Class rdf:ID="Module">
		<rdfs:subClassOf rdf:resource="#LearningObject"/>
		<rdfs:comment>This class is a direct subclass of the LearningObject class. The Module class refers to a LO which is comprised of several lessons with significant relevance and has a duration of 10 hours, at most, i.e. Overriding, Dynamic Binding and Polymorphism module of the CS252 Course of the Computer Science Department at the University of Crete.</rdfs:comment>
	</rdfs:Class>

	<rdfs:Class rdf:ID="Lesson">
		<rdfs:subClassOf rdf:resource="#LearningObject"/>
		<rdfs:comment>This class is a direct subclass of the LearningObject class and refers to a grouping of components (simple LOs) with related content that form a session of approximately 90 minutes, which is widely known as an academic lesson. Therefore, instances of this class are considered to be composite Learning Objects, i.e. a single lesson of the CS252 Course of the Computer Science Department at the University of Crete.</rdfs:comment>
	</rdfs:Class>
	
	<rdfs:Class rdf:ID="Component">
		<rdfs:subClassOf rdf:resource="#LearningObject"/>
		<rdfs:comment>This class is a direct subclass of the LearningObject class and refers to every object that might be used in the learning process, like a text file, a diagram, a table, a figure, a .ppt file an so on.  This kind of LO does not contain any other LOs and forms the first granularity level of LOs, thus it is called a simple Learning Object.</rdfs:comment>
		<rdfs:comment>Class LearningResourceType along with subclasses Exercise, Simulation, Questionnaire, Diagram, Figure, Graph, Index, Slide, Table, NarrativeText, Exam, Experiment, ProblemStatement, SelfAssessment from the IEEE LOM RDF binding file imsmd_educationalv1p2 of the IMS project map to subclasses of class Component respectively, inheriting all the properties of Class LearningObject.</rdfs:comment>
	</rdfs:Class>
	
	<rdfs:Class rdf:ID="MyTestSuperClass">
	</rdfs:Class>
	
	<rdfs:Class rdf:ID="MyTestSubClass1">
		<rdfs:subClassOf rdf:resource="#MyTestSuperClass"/>
	</rdfs:Class>
	
	<rdfs:Class rdf:ID="MyTestSubClass2">
		<rdfs:subClassOf rdf:resource="#MyTestSuperClass"/>
	</rdfs:Class>
	
	<rdfs:Class rdf:ID="MyTestSubClass3">
		<rdfs:subClassOf rdf:resource="#MyTestSubClass1"/>
	</rdfs:Class>
	
<!-- This RDF/S schema binding of IEEE LOM 1484.12.1 - 2002 was  
     developed within the SeLeNe Project IST-2001-39045 in the framework 
     of the Information Society Technology Programme, part of the Fifth  
     Research And Technological Development Framework Programme of the   
     European Community                                                  

     Copyright (c) 2003, ICS-FORTH, All Rights Reserved                  
     Version: 1.0                                                        
     Authors: 
      	      Apostolidis Apostolos <apostol@csd.uoc.gr>
              Pediaditaki Sofia     <pediadit@csd.uoc.gr> 		 -->                 
                                                                     

<!-- Classes below have been defined by IEEE LOM  -->
	

	<rdf:Property rdf:ID="description">
		<rdfs:domain rdf:resource="#LearningObject"/>
		<rdfs:range rdf:resource="http://www.w3.org/2001/XMLSchema#string"/>
		<rdfs:comment>This property provides a general description of the LO, similar to the tag "title" in a HTML file, i.e. "CS252 analyzes the main principles and characteristics of Object Oriented Programming". Corresponds to LOM.General.description.</rdfs:comment>
	</rdf:Property>

	<rdf:Property rdf:ID="title">
		<rdfs:domain rdf:resource="#LearningObject"/>
		<rdfs:range rdf:resource="http://www.w3.org/2001/XMLSchema#string"/>
		<rdfs:comment>This property provides the actual name given to this Learning Object. The values assigned may be multiple, i.e. CS252: Object Oriented Programming. Corresponds to LOM.General.Title.</rdfs:comment>
	</rdf:Property>

	<rdf:Property rdf:ID="language">
		<rdfs:domain rdf:resource="#LearningObject"/>
		<rdfs:range rdf:resource="http://www.w3.org/2001/XMLSchema#string"/>
		<rdfs:comment>The primary human language or languages used within this learning object to communicate to the intended user, i.e. "en", "gr", etc.Corresponds to LOM.General.Language.</rdfs:comment>
	</rdf:Property>

	<rdf:Property rdf:ID="keyword">
		<rdfs:domain rdf:resource="#LearningObject"/>
		<rdfs:range rdf:resource="http://www.w3.org/2001/XMLSchema#string"/>
		<rdfs:comment>A keyword or phrase describing the topic of this learning object. This data element should not be used for characteristics that can be described by other data elements, i.e. "Object Oriented Programming". Corresponds to LOM.General.keyword.</rdfs:comment>
	</rdf:Property>

	<rdf:Property rdf:ID="coverage">
		<rdfs:domain rdf:resource="#LearningObject"/>
		<rdfs:range rdf:resource="http://www.w3.org/2001/XMLSchema#string"/>
		<rdfs:comment>The time, culture, geography or region to which this learning object applies. It gives the extent or scope of the content of the learning object. Coverage will typically include spatial location (a place name or geographic coordinates), temporal period (a period label, date, or date range) or jurisdiction (such as a named administrative entity). Recommended best practice is to select a value from a controlled vocabulary (for example, the Thesaurus of Geographic Names [TGN]) and that, where appropriate, named places or time periods be used in preference to numeric identifiers such as sets of coordinates or date ranges, i.e. "University of Crete, Spring 2003, Greece". Corresponds to LOM.General.coverage.</rdfs:comment>
	</rdf:Property>
	
	<rdf:Property rdf:ID="myproperty">
		<rdfs:domain rdf:resource="#MyTestSubClass2"/>
		<rdfs:range rdf:resource="http://www.w3.org/2001/XMLSchema#string"/>
		<rdfs:comment>This is mine.</rdfs:comment>
	</rdf:Property>
	
	<rdf:Property rdf:ID="myproperty2">
		<rdfs:domain rdf:resource="#MyTestSubClass2"/>
		<rdfs:range rdf:resource="#MyTestSubClass3"/>
		<rdfs:comment>This is mine.</rdfs:comment>
	</rdf:Property>
	
<!-- This RDF/S schema binding of IEEE LOM 1484.12.1 - 2002 was  
     developed within the SeLeNe Project IST-2001-39045 in the framework 
     of the Information Society Technology Programme, part of the Fifth  
     Research And Technological Development Framework Programme of the   
     European Community                                                  

     Copyright (c) 2003, ICS-FORTH, All Rights Reserved                  
     Version: 1.0                                                        
     Authors: 
      	      Apostolidis Apostolos <apostol@csd.uoc.gr>
	      Pediaditaki Sofia     <pediadit@csd.uoc.gr> 		 -->

		      
     <!--    ALL PROPERTIES BELOW CORRESPOND TO LOM.GENERAL CATEGORY     -->

</rdf:RDF>

